theories/zoo_saturn/mpmc_queue_2.v
@@ -9,6 +9,8 @@ From zoo.iris.base_logic Require Import
   lib.auth_nat_max.
 From zoo.language Require Import
   notations.
+From zoo.program_logic Require Import
+  typed_prophet.
 From zoo.diaframe Require Import
   diaframe.
 From zoo_std Require Import
@@ -21,10 +23,29 @@ From zoo_saturn Require Import
 From zoo Require Import
   options.
 
-Implicit Types l back : location.
+Implicit Types l back prev_back : location.
 Implicit Types backs : gmap location nat.
-Implicit Types v t : val.
-Implicit Types vs move : list val.
+Implicit Types v w t pref suff 𝑚𝑜𝑣𝑒 : val.
+Implicit Types vs vs_front vs_back move : list val.
+
+#[local] Program Definition prophet := {|
+  typed_strong_prophet1_type :=
+    bool ;
+  typed_strong_prophet1_of_val v _ :=
+    match v with
+    | ValBool b =>
+        Some b
+    | _ =>
+        None
+    end ;
+  typed_strong_prophet1_to_val b :=
+    (#b, inhabitant) ;
+|}.
+Solve Obligations of prophet with
+  try done.
+Next Obligation.
+  naive_solver.
+Qed.
 
 Inductive emptiness :=
   | Empty
@@ -34,103 +55,103 @@ Implicit Types empty : emptiness.
 #[local] Instance emptiness_inhabited : Inhabited emptiness :=
   populate Empty.
 
-Inductive lstatus :=
+Inductive status :=
   | Stable empty
   | Unstable back move.
-Implicit Types lstatus : lstatus.
+Implicit Types status : status.
 
-#[local] Instance lstatus_inhabited : Inhabited lstatus :=
+#[local] Instance status_inhabited : Inhabited status :=
   populate (Stable inhabitant).
 
-Record lstate := {
-  lstate_backs : gmap location nat ;
-  lstate_index : nat ;
-  lstate_lstatus : lstatus ;
+Record state := {
+  state_backs : gmap location nat ;
+  state_index : nat ;
+  state_status : status ;
 }.
-Implicit Types lstate : lstate.
+Implicit Types state : state.
 
-#[local] Definition lstate_with_lstatus lstate lstatus :=
-  {|lstate_backs := lstate.(lstate_backs) ;
-    lstate_index := lstate.(lstate_index) ;
-    lstate_lstatus := lstatus ;
+#[local] Definition state_with_status state status :=
+  {|state_backs := state.(state_backs) ;
+    state_index := state.(state_index) ;
+    state_status := status ;
   |}.
 
-#[local] Definition lstate_le lstate1 lstate2 :=
-  lstate1.(lstate_backs) ⊆ lstate2.(lstate_backs) ∧
-  lstate1.(lstate_index) ≤ lstate2.(lstate_index).
+#[local] Definition state_le state1 state2 :=
+  state1.(state_backs) ⊆ state2.(state_backs) ∧
+  state1.(state_index) ≤ state2.(state_index).
 
-#[local] Instance lstate_inhabited : Inhabited lstate :=
+#[local] Instance state_inhabited : Inhabited state :=
   populate {|
-    lstate_backs := inhabitant ;
-    lstate_index := inhabitant ;
-    lstate_lstatus := inhabitant ;
+    state_backs := inhabitant ;
+    state_index := inhabitant ;
+    state_status := inhabitant ;
   |}.
 
-#[local] Instance lstate_le_reflexive :
-  Reflexive lstate_le.
+#[local] Instance state_le_reflexive :
+  Reflexive state_le.
 Proof.
   done.
 Qed.
-#[local] Instance lstate_le_transitive :
-  Transitive lstate_le.
+#[local] Instance state_le_transitive :
+  Transitive state_le.
 Proof.
-  intros lstate1 lstate2 lstate3 (? & ?) (? & ?).
+  intros state1 state2 state3 (? & ?) (? & ?).
   split.
   - etrans; done.
   - lia.
 Qed.
 
-Inductive lstep : relation lstate :=
-  | lstep_empty lstate1 lstate2 :
-      lstate1.(lstate_lstatus) = Stable Nonempty →
-      lstate2 = lstate_with_lstatus lstate1 (Stable Empty) →
-      lstep lstate1 lstate2
-  | lstep_destabilize lstate1 lstate2 back move :
-      lstate1.(lstate_lstatus) = Stable Empty →
-      lstate2 = lstate_with_lstatus lstate1 (Unstable back move) →
-      lstep lstate1 lstate2
-  | lstep_stabilize lstate1 lstate2 back move :
-      lstate1.(lstate_lstatus) = Unstable back move →
-      back ∉ dom lstate1.(lstate_backs) →
-      lstate2 =
-        {|lstate_backs := <[back := lstate1.(lstate_index) + length move]> lstate1.(lstate_backs) ;
-          lstate_index := lstate1.(lstate_index) + length move ;
-          lstate_lstatus := Stable Nonempty ;
+Inductive step : relation state :=
+  | step_empty state1 state2 :
+      state1.(state_status) = Stable Nonempty →
+      state2 = state_with_status state1 (Stable Empty) →
+      step state1 state2
+  | step_destabilize state1 state2 back move :
+      state1.(state_status) = Stable Empty →
+      state2 = state_with_status state1 (Unstable back move) →
+      step state1 state2
+  | step_stabilize state1 state2 back move :
+      state1.(state_status) = Unstable back move →
+      state1.(state_backs) !! back = None →
+      state2 =
+        {|state_backs := <[back := state1.(state_index) + length move]> state1.(state_backs) ;
+          state_index := state1.(state_index) + length move ;
+          state_status := Stable Nonempty ;
         |} →
-      lstep lstate1 lstate2.
-#[local] Hint Constructors lstep : core.
+      step state1 state2.
+#[local] Hint Constructors step : core.
 
-#[local] Definition lsteps :=
-  rtc lstep.
+#[local] Definition steps :=
+  rtc step.
 
-#[local] Lemma lstep_mono lstate1 lstate2 :
-  lstep lstate1 lstate2 →
-  lstate_le lstate1 lstate2.
+#[local] Lemma step_mono state1 state2 :
+  step state1 state2 →
+  state_le state1 state2.
 Proof.
-  intros Hlstep. invert Hlstep; [done.. |].
+  intros Hstep. invert Hstep; [done.. |].
   split.
-  - apply insert_subseteq, not_elem_of_dom. done.
+  - apply insert_subseteq. done.
   - simpl. lia.
 Qed.
-#[local] Lemma lsteps_mono lstate1 lstate2 :
-  lsteps lstate1 lstate2 →
-  lstate_le lstate1 lstate2.
+#[local] Lemma steps_mono state1 state2 :
+  steps state1 state2 →
+  state_le state1 state2.
 Proof.
-  intros Hlsteps.
+  intros Hsteps.
   rewrite -preorder_rtc.
-  apply (rtc_congruence (R := lstep) id); last done.
-  apply lstep_mono.
+  apply (rtc_congruence (R := step) id); last done.
+  apply step_mono.
 Qed.
 
 Class MpmcQueue2G Σ `{zoo_G : !ZooG Σ} := {
   #[local] mpmc_queue_2_G_model_G :: TwinsG Σ (leibnizO (list val)) ;
-  #[local] mpmc_queue_2_G_lstate_G :: AuthMonoG (A := leibnizO lstate) Σ lstep ;
+  #[local] mpmc_queue_2_G_state_G :: AuthMonoG (A := leibnizO state) Σ step ;
   #[local] mpmc_queue_2_G_front_G :: AuthNatMaxG Σ ;
 }.
 
 Definition mpmc_queue_2_Σ := #[
   twins_Σ (leibnizO (list val)) ;
-  auth_mono_Σ (A := leibnizO lstate) lstep ;
+  auth_mono_Σ (A := leibnizO state) step ;
   auth_nat_max_Σ
 ].
 #[global] Instance subG_mpmc_queue_2_Σ Σ `{zoo_G : !ZooG Σ} :
@@ -140,28 +161,82 @@ Proof.
   solve_inG.
 Qed.
 
-#[local] Fixpoint suffix_to_val (i : nat) vs :=
+#[local] Fixpoint suffix_to_val (i : nat) vs : val :=
   match vs with
   | [] =>
-      ‘Front( #i )%V
+      ‘Front[ #i ]
   | v :: vs =>
-      ‘Cons( #i, v, suffix_to_val (S i) vs )%V
+      ‘Cons[ #i, v, suffix_to_val (S i) vs ]
   end.
 
-#[local] Fixpoint prefix_to_val (i : nat) back vs :=
+#[local] Lemma suffix_to_val_generative i1 vs1 i2 vs2 :
+  suffix_to_val i1 vs1 ≈ suffix_to_val i2 vs2 →
+  suffix_to_val i1 vs1 = suffix_to_val i2 vs2.
+Proof.
+  destruct vs1 as [| v1 vs1], vs2 as [| v2 vs2] => Hsimilar.
+  all: zoo_simpl.
+  all: congruence.
+Qed.
+
+#[local] Instance suffix_to_val_inj2 :
+  Inj2 (=) (=) (=) suffix_to_val.
+Proof.
+  move=> + vs1. induction vs1 as [| v1 vs1 IH] => i1 i2 [| v2 vs2] Hsimilar.
+  all: naive_solver.
+Qed.
+#[local] Instance suffix_to_val_inj2' :
+  Inj2 (=) (=) (≈) suffix_to_val.
+Proof.
+  intros ?* Hsimilar%suffix_to_val_generative.
+  apply (inj2 suffix_to_val). done.
+Qed.
+
+#[local] Fixpoint prefix_to_val (i : nat) back vs : val :=
   match vs with
   | [] =>
       #back
   | v :: vs =>
-      ‘Snoc( #(i + length vs), v, prefix_to_val i back vs )%V
+      ‘Snoc[ #⁺(i + length vs), v, prefix_to_val i back vs ]
   end.
+
+#[local] Lemma prefix_to_val_generative i1 back1 vs1 i2 back2 vs2 :
+  prefix_to_val i1 back1 vs1 ≈ prefix_to_val i2 back2 vs2 →
+  prefix_to_val i1 back1 vs1 = prefix_to_val i2 back2 vs2.
+Proof.
+  destruct vs1 as [| v1 vs1], vs2 as [| v2 vs2] => Hsimilar.
+  all: zoo_simpl.
+  all: congruence.
+Qed.
+
+#[local] Lemma prefix_to_val_inj3 i1 back1 vs1 i2 back2 vs2 :
+  prefix_to_val i1 back1 vs1 = prefix_to_val i2 back2 vs2 →
+    (vs1 ≠ [] → i1 = i2) ∧
+    back1 = back2 ∧
+    vs1 = vs2.
+Proof.
+  move: i1 i2 vs2. induction vs1 as [| v1 vs1 IH] => i1 i2 [| v2 vs2] /= Hsimilar.
+  all: zoo_simpl; try done.
+  edestruct IH as (_ & -> & Hvs); first done.
+  rewrite {}Hvs in Hsimilar |- *.
+  auto with lia.
+Qed.
+#[local] Lemma prefix_to_val_inj3' i1 back1 vs1 i2 back2 vs2 :
+  prefix_to_val i1 back1 vs1 ≈ prefix_to_val i2 back2 vs2 →
+    (vs1 ≠ [] → i1 = i2) ∧
+    back1 = back2 ∧
+    vs1 = vs2.
+Proof.
+  intros Hsimilar%prefix_to_val_generative.
+  apply prefix_to_val_inj3. done.
+Qed.
 
 Section mpmc_queue_2_G.
   Context `{mpmc_queue_2_G : MpmcQueue2G Σ}.
 
   Record metadata := {
+    metadata_inv : namespace ;
     metadata_model : gname ;
-    metadata_lstate : gname ;
+    metadata_state : gname ;
     metadata_front : gname ;
   }.
   Implicit Types γ : metadata.
@@ -183,19 +258,19 @@ Section mpmc_queue_2_G.
   #[local] Definition model₂ γ :=
     model₂' γ.(metadata_model).
 
-  #[local] Definition lstate_auth' γ_lstate backs i lstatus :=
-    auth_mono_auth _ γ_lstate (DfracOwn 1)
-      {|lstate_backs := backs ;
-        lstate_index := i ;
-        lstate_lstatus := lstatus ;
+  #[local] Definition state_auth' γ_state backs i status :=
+    auth_mono_auth _ γ_state (DfracOwn 1)
+      {|state_backs := backs ;
+        state_index := i ;
+        state_status := status ;
       |}.
-  #[local] Definition lstate_auth γ backs i lstatus :=
-    lstate_auth' γ.(metadata_lstate) backs i lstatus.
-  #[local] Definition lstate_lb γ backs i lstatus :=
-    auth_mono_lb _ γ.(metadata_lstate)
-      {|lstate_backs := backs ;
-        lstate_index := i ;
-        lstate_lstatus := lstatus ;
+  #[local] Definition state_auth γ backs i status :=
+    state_auth' γ.(metadata_state) backs i status.
+  #[local] Definition state_lb γ backs i status :=
+    auth_mono_lb _ γ.(metadata_state)
+      {|state_backs := backs ;
+        state_index := i ;
+        state_status := status ;
       |}.
 
   #[local] Definition front_auth' γ_front i :=
@@ -205,43 +280,88 @@ Section mpmc_queue_2_G.
   #[local] Definition front_lb γ i :=
     auth_nat_max_lb γ.(metadata_front) i.
 
-  #[local] Definition back_model back (i : nat) v_move : iProp Σ :=
+  #[local] Definition back_model_1 back (i : nat) : iProp Σ :=
     back ↦ₕ Header §Back 2 ∗
-    back.[index] ↦□ #i ∗
-    back.[move] ↦ v_move.
-  #[local] Definition back_model' back i : iProp Σ :=
-    ∃ v_move,
-    back_model back i v_move.
+    back.[index] ↦□ #i.
+  #[local] Instance : CustomIpatFormat "back_model_1" :=
+    "(
+      #Hback{}_header &
+      #Hback{}_index
+    )".
+  #[local] Definition back_model_2 back (i : nat) 𝑚𝑜𝑣𝑒 : iProp Σ :=
+    back_model_1 back i ∗
+    back.[move] ↦ 𝑚𝑜𝑣𝑒.
+  #[local] Instance : CustomIpatFormat "back_model_2" :=
+    "(
+      { {only_move} _
+      ; (:back_model_1 //)
+      } &
+      Hback{}_move{_{suff}}
+    )".
+  #[local] Definition back_model_3 back i : iProp Σ :=
+    ∃ 𝑚𝑜𝑣𝑒,
+    back_model_2 back i 𝑚𝑜𝑣𝑒.
+  #[local] Instance : CustomIpatFormat "back_model_3" :=
+    "(
+      %𝑚𝑜𝑣𝑒{} &
+      (:back_model_2 {//} {/only_move/})
+    )".
+
+  #[local] Definition inv_status_stable backs i vs_front i_back back vs_back vs empty : iProp Σ :=
+    ⌜i_back = i⌝ ∗
+    ⌜backs !! back = Some i_back⌝ ∗
+    ⌜vs = vs_front ++ reverse vs_back⌝ ∗
+    ⌜if empty then vs_front = [] else 0 < length vs_front⌝.
+  #[local] Instance : CustomIpatFormat "inv_status_stable" :=
+    "(
+      -> &
+      %Hbacks{}_lookup &
+      %Hvs{} &
+      {{empty}->;%}
+    )".
+  #[local] Definition inv_status_unstable backs i vs_front i_back back vs_back vs back_ move : iProp Σ :=
+    ∃ prev_back,
+    ⌜back_ = back⌝ ∗
+    ⌜backs !! prev_back = Some i⌝ ∗
+    ⌜i_back = (i + length move)%nat⌝ ∗
+    ⌜vs_front = []⌝ ∗
+    ⌜vs_back = []⌝ ∗
+    ⌜vs = reverse move⌝ ∗
+    back_model_2 back i_back (prefix_to_val i prev_back move).
+  #[local] Instance : CustomIpatFormat "inv_status_unstable" :=
+    "(
+      %prev_back{_{}} &
+      -> &
+      %Hbacks{}_lookup &
+      -> &
+      {{lazy}%Hvs_front{};->} &
+      -> &
+      -> &
+      Hback{}
+    )".
+  #[local] Definition inv_status backs i status vs_front i_back back vs_back vs : iProp Σ :=
+    match status with
+    | Stable empty =>
+        inv_status_stable backs i vs_front i_back back vs_back vs empty
+    | Unstable back_ move =>
+        inv_status_unstable backs i vs_front i_back back vs_back vs back_ move
+    end.
 
   #[local] Definition inv_inner l γ : iProp Σ :=
-    ∃ backs i lstatus i_front vs_front i_back back vs_back vs,
+    ∃ backs i status i_front vs_front i_back back vs_back vs,
     l.[front] ↦ suffix_to_val i_front vs_front ∗
     front_auth γ i_front ∗
-    l.[back] ↦ prefix_to_val i_back back vs_front ∗
-    ([∗ map] back ↦ i ∈ backs, back_model' back i) ∗
+    l.[back] ↦ prefix_to_val (S i_back) back vs_back ∗
+    ([∗ map] back ↦ i ∈ backs, back_model_3 back i) ∗
     model₂ γ vs ∗
-    lstate_auth γ backs i lstatus ∗
+    state_auth γ backs i status ∗
     ⌜(i_front + length vs_front)%nat = S i⌝ ∗
-    match lstatus with
-    | Stable empty =>
-        ⌜i_back = i⌝ ∗
-        ⌜backs !! back = Some i_back⌝ ∗
-        ⌜vs = vs_front ++ reverse vs_back⌝ ∗
-        ⌜if empty then vs_front = [] else 0 < length vs_front⌝
-    | Unstable back_ move =>
-        ∃ back',
-        ⌜back_ = back⌝ ∗
-        ⌜backs !! back' = Some i⌝ ∗
-        ⌜i_back = (i + length move)%nat⌝ ∗
-        ⌜vs_front = []⌝ ∗
-        ⌜vs_back = []⌝ ∗
-        back_model back i_back (prefix_to_val i back' move)
-    end.
+    inv_status backs i status vs_front i_back back vs_back vs.
   #[local] Instance : CustomIpatFormat "inv_inner" :=
     "(
       %backs{} &
       %i{} &
-      %lstatus{} &
+      %status{} &
       %i_front{} &
       %vs_front{} &
       %i_back{} &
@@ -253,36 +373,23 @@ Section mpmc_queue_2_G.
       Hl_back &
       Hbacks &
       Hmodel₂ &
-      >Hlstate_auth &
-      >% &
-      Hlstatus
+      >Hstate_auth &
+      >%Hi{} &
+      Hstatus
     )".
-  #[local] Instance : CustomIpatFormat "inv_inner_stable" :=
-    "(
-      % &
-      %Hbacks_lookup &
-      % &
-      %
-    )".
-  #[local] Instance : CustomIpatFormat "inv_inner_unstable" :=
-    "(
-      %back' &
-      % &
-      %Hbacks_lookup &
-      % &
-      % &
-      % &
-      Hback
-    )".
+  #[local] Definition inv' l γ : iProp Σ :=
+    inv γ.(metadata_inv) (inv_inner l γ).
   Definition mpmc_queue_2_inv t ι : iProp Σ :=
     ∃ l γ,
     ⌜t = #l⌝ ∗
+    ⌜ι = γ.(metadata_inv)⌝ ∗
     meta l nroot γ ∗
-    inv ι (inv_inner l γ).
+    inv' l γ.
   #[local] Instance : CustomIpatFormat "inv" :=
     "(
       %l &
       %γ &
+      -> &
       -> &
       #Hmeta &
       #Hinv
@@ -295,10 +402,10 @@ Section mpmc_queue_2_G.
     model₁ γ vs.
   #[local] Instance : CustomIpatFormat "model" :=
     "(
-      %l &
-      %γ &
-      -> &
-      #Hmeta &
+      %l_ &
+      %γ_ &
+      %Heq &
+      #Hmeta_ &
       Hmodel₁
     )".
 
@@ -313,30 +420,217 @@ Section mpmc_queue_2_G.
     apply _.
   Qed.
 
-  #[local] Lemma lstate_lb_valid γ backs1 i1 lstatus1 backs2 i2 lstatus2 :
-    lstate_auth γ backs1 i1 lstatus1 -∗
-    lstate_lb γ backs2 i2 lstatus2 -∗
+  #[local] Lemma model_alloc :
+    ⊢ |==>
+      ∃ γ_model,
+      model₁' γ_model [] ∗
+      model₂' γ_model [].
+  Proof.
+    apply twins_alloc'.
+  Qed.
+  #[local] Lemma model_agree γ vs1 vs2 :
+    model₁ γ vs1 -∗
+    model₂ γ vs2 -∗
+    ⌜vs1 = vs2⌝.
+  Proof.
+    apply: twins_agree_L.
+  Qed.
+  #[local] Lemma model_update {γ vs1 vs2} vs :
+    model₁ γ vs1 -∗
+    model₂ γ vs2 ==∗
+      model₁ γ vs ∗
+      model₂ γ vs.
+  Proof.
+    apply twins_update'.
+  Qed.
+
+  #[local] Lemma state_alloc back :
+    ⊢ |==>
+      ∃ γ_state,
+      state_auth' γ_state {[back := 0]} 0 (Stable Empty).
+  Proof.
+    apply auth_mono_alloc.
+  Qed.
+  #[local] Lemma state_lb_get γ backs i status :
+    state_auth γ backs i status ⊢
+    state_lb γ backs i status.
+  Proof.
+    apply auth_mono_lb_get.
+  Qed.
+  #[local] Lemma state_lb_valid γ backs1 i1 status1 backs2 i2 status2 :
+    state_auth γ backs1 i1 status1 -∗
+    state_lb γ backs2 i2 status2 -∗
       ⌜backs2 ⊆ backs1⌝ ∗
       ⌜i2 ≤ i2⌝.
   Proof.
     iIntros "Hauth Hlb".
-    iDestruct (auth_mono_lb_valid with "Hauth Hlb") as %(? & ?)%lsteps_mono. done.
+    iDestruct (auth_mono_lb_valid with "Hauth Hlb") as %(? & ?)%steps_mono. done.
   Qed.
-  #[local] Lemma lstate_lb_header l γ ι backs i lstatus back :
-    back ∈ dom backs →
-    inv ι (inv_inner l γ) -∗
-    lstate_lb γ backs i lstatus -∗
-      |={⊤}=>
-      back ↦ₕ Header §Back 2.
+  #[local] Lemma state_lb_stabilized γ backs1 i1 status1 backs2 i2 back2 move2 :
+    ( status1 ≠ Unstable back2 move2
+    ∨ i2 + length move2 ≤ i1 ∧
+      0 < length move2
+    ) →
+    state_auth γ backs1 i1 status1 -∗
+    state_lb γ backs2 i2 (Unstable back2 move2) -∗
+    ⌜backs1 !! back2 = Some (i2 + length move2)%nat⌝.
   Proof.
-    iIntros ((j & Hbacks_lookup)%elem_of_dom) "#Hinv #Hlstate_lb".
-    iInv "Hinv" as "(:inv_inner =')".
-    iAssert (▷ back ↦ₕ Header §Back 2)%I as "#>$".
-    { iDestruct (lstate_lb_valid with "Hlstate_auth Hlstate_lb") as %(? & _).
-      iDestruct (big_sepM_lookup with "Hbacks") as "(%v_move & $ & _)".
+    iIntros "%H Hauth Hlb".
+    iDestruct (auth_mono_lb_valid with "Hauth Hlb") as %[? | (step3 & Hstep & (? & _)%steps_mono)]%rtc_inv.
+    all: iPureIntro.
+    - naive_solver lia.
+    - invert Hstep.
+      eapply lookup_weaken; last done.
+      rewrite lookup_insert //.
+  Qed.
+  #[local] Lemma state_lb_unstabilized γ backs1 i1 status1 backs2 i2 back2 move2 :
+    i1 < i2 + length move2 →
+    state_auth γ backs1 i1 status1 -∗
+    state_lb γ backs2 i2 (Unstable back2 move2) -∗
+      ⌜backs1 = backs2⌝ ∗
+      ⌜i1 = i2⌝ ∗
+      ⌜status1 = Unstable back2 move2⌝.
+  Proof.
+    iIntros "%H Hauth Hlb".
+    iDestruct (auth_mono_lb_valid with "Hauth Hlb") as %[? | (step3 & Hstep & (_ & HH2)%steps_mono)]%rtc_inv.
+    all: iPureIntro.
+    - simplify. done.
+    - invert Hstep. lia.
+  Qed.
+  #[local] Lemma state_stabilize γ backs i back move :
+    backs !! back = None →
+    state_auth γ backs i (Unstable back move) ⊢ |==>
+      state_auth γ (<[back := i + length move]> backs) (i + length move) (Stable Nonempty) ∗
+      state_lb γ (<[back := i + length move]> backs) (i + length move) (Stable Nonempty).
+  Proof.
+    iIntros "%Hbacks_lookup Hauth".
+    iMod (auth_mono_update' with "Hauth") as "Hauth"; first eauto.
+    iDestruct (state_lb_get with "Hauth") as "#Hstate_lb".
+    iSteps.
+  Qed.
+
+  #[local] Lemma front_alloc :
+    ⊢ |==>
+      ∃ γ_front,
+      front_auth' γ_front 1.
+  Proof.
+    apply auth_nat_max_alloc.
+  Qed.
+  #[local] Lemma front_lb_get γ i :
+    front_auth γ i ⊢
+    front_lb γ i.
+  Proof.
+    apply auth_nat_max_lb_get.
+  Qed.
+  #[local] Lemma front_lb_valid γ i1 i2 :
+    front_auth γ i1 -∗
+    front_lb γ i2 -∗
+    ⌜i2 ≤ i1⌝.
+  Proof.
+    apply auth_nat_max_lb_valid.
+  Qed.
+  #[local] Lemma front_update γ i :
+    front_auth γ i ⊢ |==>
+    front_auth γ (S i).
+  Proof.
+    apply auth_nat_max_update. lia.
+  Qed.
+
+  #[local] Lemma inv'_back_model_1 {l γ backs i status} back i_back :
+    backs !! back = Some i_back →
+    inv' l γ -∗
+    state_lb γ backs i status ={⊤}=∗
+    back_model_1 back i_back.
+  Proof.
+    iIntros "%Hbacks_lookup #Hinv #Hstate_lb".
+    iInv "Hinv" as "(:inv_inner =1)".
+    iAssert (▷ back_model_1 back i_back)%I as "#>$".
+    { iDestruct (state_lb_valid with "Hstate_auth Hstate_lb") as %(? & _).
+      iDestruct (big_sepM_lookup with "Hbacks") as "(:back_model_3)".
       { eapply lookup_weaken; done. }
+      iFrame "#".
     }
     iFrameSteps.
+  Qed.
+
+  #[local] Lemma mpmc_queue_2_suffix_index_spec (i : nat) vs :
+    {{{
+      True
+    }}}
+      mpmc_queue_2_suffix_index (suffix_to_val i vs)
+    {{{
+      RET #i;
+      True
+    }}}.
+  Proof.
+    destruct vs; iSteps.
+  Qed.
+
+  #[local] Lemma mpmc_queue_2_prefix_index_spec (i : nat) back vs :
+    {{{
+      back ↦ₕ Header §Back 2 ∗
+      back.[index] ↦□ #i
+    }}}
+      mpmc_queue_2_prefix_index (prefix_to_val (S i) back vs)
+    {{{
+      RET #⁺(i + length vs);
+      True
+    }}}.
+  Proof.
+    iIntros "%Φ (#Hback_header & #Hback_index) HΦ".
+
+    wp_rec.
+    destruct vs => /=.
+    1: rewrite Nat.add_0_r.
+    2: rewrite Nat.add_succ_r.
+    all: iSteps.
+  Qed.
+
+  #[local] Lemma mpmc_queue_2_rev_0_spec i vs1 vs2 back :
+    0 < length vs1 →
+    {{{
+      back ↦ₕ Header §Back 2
+    }}}
+      mpmc_queue_2_rev_0 (suffix_to_val (S i + length vs2) vs1) (prefix_to_val (S i) back vs2)
+    {{{
+      RET suffix_to_val (S i) (reverse vs2 ++ vs1);
+      True
+    }}}.
+  Proof.
+    iIntros "%Hvs1 %Φ #Hback_header HΦ".
+
+    iInduction vs2 as [| v2 vs2] "IH" forall (vs1 Hvs1).
+    all: wp_rec.
+    all: destruct vs1 as [| v1 vs1]; first naive_solver lia.
+    all: wp_pures.
+
+    - rewrite Nat.add_0_r. iSteps.
+
+    - rewrite Nat.add_succ_r.
+      wp_apply ("IH" $! (v2 :: v1 :: vs1) with "[%]").
+      { simpl. lia. }
+      rewrite reverse_cons -assoc //.
+  Qed.
+  #[local] Lemma mpmc_queue_2_rev_spec i back vs :
+    0 < length vs →
+    {{{
+      back ↦ₕ Header §Back 2
+    }}}
+      mpmc_queue_2_rev (prefix_to_val (S i) back vs)
+    {{{
+      RET suffix_to_val (S i) (reverse vs);
+      True
+    }}}.
+  Proof.
+    iIntros "%Hvs %Φ #Hback_header HΦ".
+
+    wp_rec.
+    destruct vs as [| v vs]; first naive_solver lia.
+    wp_pures.
+    replace (⁺(S (i + length vs)) + 1)%Z with ⁺(S (S (i + length vs))) by lia.
+    wp_apply (mpmc_queue_2_rev_0_spec i [v] with "Hback_header").
+    { simpl. lia. }
+    rewrite reverse_cons //.
   Qed.
 
   Lemma mpmc_queue_2_create_spec ι :
@@ -350,7 +644,52 @@ Section mpmc_queue_2_G.
       mpmc_queue_2_model t []
     }}}.
   Proof.
-  Admitted.
+    iIntros "%Φ _ HΦ".
+
+    wp_rec.
+    wp_block back as "Hback_header" "_" "(Hback_index & Hback_move & _)".
+    iMod (pointsto_persist with "Hback_index") as "#Hback_index".
+    wp_block l as "Hmeta" "(Hl_front & Hl_back & _)".
+
+    iMod model_alloc as "(%γ_model & Hmodel₁ & Hmodel₂)".
+    iMod (state_alloc back) as "(%γ_state & Hstate_auth)".
+    iMod front_alloc as "(%γ_front & Hfront_auth)".
+
+    pose γ := {|
+      metadata_inv := ι ;
+      metadata_model := γ_model ;
+      metadata_state := γ_state ;
+      metadata_front := γ_front ;
+    |}.
+    iMod (meta_set γ with "Hmeta") as "#Hmeta"; first done.
+
+    iApply "HΦ".
+    iSplitR "Hmodel₁"; last iSteps.
+    iExists l, γ. iStep 3. iApply inv_alloc.
+    iExists {[back := 0]}, 0, (Stable Empty), 1, [], 0, back, [], [].
+    rewrite /= /inv_status_stable big_sepM_singleton lookup_singleton.
+    iFrameSteps.
+  Qed.
+
+  #[local] Lemma front_spec l γ :
+    {{{
+      inv' l γ
+    }}}
+      (#l).{front}
+    {{{ i_front vs_front,
+      RET suffix_to_val i_front vs_front;
+      front_lb γ i_front
+    }}}.
+  Proof.
+    iIntros "%Φ Hinv HΦ".
+
+    wp_bind (_.{front})%E.
+    iInv "Hinv" as "(:inv_inner)".
+    wp_load.
+    iDestruct (front_lb_get with "Hfront_auth") as "#Hfront_lb".
+    iSplitR "HΦ". { iFrameSteps. }
+    iSteps.
+  Qed.
 
   Lemma mpmc_queue_2_size_spec t ι :
     <<<
@@ -365,7 +704,75 @@ Section mpmc_queue_2_G.
       True
     >>>.
   Proof.
-  Admitted.
+    iIntros "%Φ (:inv) HΦ".
+
+    iLöb as "HLöb".
+
+    wp_rec.
+    wp_apply (front_spec with "Hinv") as (i_front1 vs_front1) "#Hfront_lb_1".
+
+    wp_smart_apply (typed_strong_prophet1_wp_proph prophet with "[//]") as (pid proph) "Hproph".
+    wp_pures.
+
+    wp_bind (_.{back})%E.
+    iInv "Hinv" as "(:inv_inner =2)".
+    wp_load.
+    destruct proph.
+
+    - iDestruct (front_lb_valid with "Hfront_auth Hfront_lb_1") as %Hi_front2.
+      iDestruct (front_lb_get with "Hfront_auth") as "#Hfront_lb_2".
+
+      iAssert (back_model_1 back2 i_back2) as "#(:back_model_1 =2)".
+      { destruct status2.
+        - iDestruct "Hstatus" as "(:inv_status_stable =2)".
+          iDestruct (big_sepM_lookup with "Hbacks") as "(:back_model_3 =2)"; first done.
+          iFrame "#".
+        - iDestruct "Hstatus" as "(:inv_status_unstable =2)".
+          iDestruct "Hback2" as "(:back_model_2 =2)".
+          iFrame "#".
+      }
+
+      iMod "HΦ" as "(%vs & (:model) & _ & HΦ)". injection Heq as <-.
+      iDestruct (meta_agree with "Hmeta Hmeta_") as %<-. iClear "Hmeta_".
+      iDestruct (model_agree with "Hmodel₁ Hmodel₂") as %->.
+      iMod ("HΦ" with "[Hmodel₁] [//]") as "HΦ"; first iSteps.
+      iAssert ⌜(i_front2 + length vs2 = i_back2 + length vs_back2 + 1)%nat⌝%I as %Hsize.
+      { destruct status2.
+        - iDestruct "Hstatus" as "(:inv_status_stable =2)". iPureIntro.
+          apply (f_equal length) in Hvs2. simpl_length in Hvs2. lia.
+        - iDestruct "Hstatus" as "(:inv_status_unstable =2)". iPureIntro.
+          simpl_length/=. lia.
+      }
+
+      iSplitR "Hproph HΦ". { iFrameSteps. }
+      iModIntro. clear- Hi_front2 Hsize.
+
+      wp_pures.
+
+      wp_bind (_.{front})%E.
+      iInv "Hinv" as "(:inv_inner =3)".
+      wp_load.
+      iDestruct (front_lb_valid with "Hfront_auth Hfront_lb_2") as %Hi_front3.
+      iSplitR "Hproph HΦ". { iFrameSteps. }
+      iModIntro. clear- Hi_front2 Hi_front3 Hsize.
+
+      wp_apply (typed_strong_prophet1_wp_resolve with "Hproph"); first done.
+      wp_equal as _ | (-> & ->)%(inj2 _); first iSteps.
+      iStep 5.
+      wp_apply (mpmc_queue_2_suffix_index_spec with "[//]") as "_".
+      wp_apply (mpmc_queue_2_prefix_index_spec with "[$]") as "_".
+      wp_pures.
+
+      replace (⁺(i_back2 + length vs_back2) - i_front1 + 1)%Z with ⁺(length vs2) by lia.
+      iSteps.
+
+    - iSplitR "Hproph HΦ". { iFrameSteps. }
+      iIntros "!> {%}".
+
+      wp_smart_apply (front_spec with "Hinv") as (i_front3 vs_front3) "_".
+      wp_apply (typed_strong_prophet1_wp_resolve with "Hproph"); first done.
+      wp_equal; iSteps.
+  Qed.
 
   Lemma mpmc_queue_2_is_empty_spec t ι :
     <<<
@@ -380,14 +787,21 @@ Section mpmc_queue_2_G.
       True
     >>>.
   Proof.
-  Admitted.
+    iIntros "%Φ #Hinv HΦ".
 
-  #[local] Lemma mpmc_queue_2_finish_spec l γ ι backs i lstatus back :
-    back ∈ dom backs →
+    wp_rec.
+
+    awp_apply (mpmc_queue_2_size_spec with "Hinv").
+    iApply (aacc_aupd_commit with "HΦ"); first done. iIntros "%vs Hmodel".
+    iAaccIntro with "Hmodel"; iSteps.
+    destruct vs; iSteps.
+  Qed.
+
+  #[local] Lemma mpmc_queue_2_finish_spec {l γ backs i status} i_back back :
+    backs !! back = Some i_back →
     {{{
-      meta l nroot γ ∗
-      inv ι (inv_inner l γ) ∗
-      lstate_lb γ backs i lstatus
+      inv' l γ ∗
+      state_lb γ backs i status
     }}}
       mpmc_queue_2_finish #back
     {{{
@@ -395,23 +809,141 @@ Section mpmc_queue_2_G.
       True
     }}}.
   Proof.
-    iIntros "%Hback %Φ (#Hmeta & #Hinv & #Hlstate_lb) HΦ".
-
-    iMod (lstate_lb_header with "Hinv Hlstate_lb") as "#Hback_header"; first done.
-    apply elem_of_dom in Hback as (j & Hbacks_lookup).
+    iIntros "%Hbacks_lookup %Φ (#Hinv & #Hstate_lb) HΦ".
+    iMod (inv'_back_model_1 with "Hinv Hstate_lb") as "(:back_model_1)"; first done.
 
     wp_rec. wp_match.
 
-    iInv "Hinv" as "(:inv_inner =')".
-    iDestruct (lstate_lb_valid with "Hlstate_auth Hlstate_lb") as %(? & _).
-    iDestruct (big_sepM_lookup_acc with "Hbacks") as "((%v_move & (_ & Hback_index & Hback_move)) & Hbacks)".
+    iInv "Hinv" as "(:inv_inner =1)".
+    iDestruct (state_lb_valid with "Hstate_auth Hstate_lb") as %(? & _).
+    iDestruct (big_sepM_lookup_acc with "Hbacks") as "((:back_model_3 only_move=) & Hbacks)".
     { eapply lookup_weaken; done. }
     wp_store.
-    iDestruct ("Hbacks" with "[$Hback_index Hback_move]") as "Hbacks"; first iSteps.
+    iDestruct ("Hbacks" with "[$]") as "Hbacks".
     iFrameSteps.
   Qed.
 
-  Lemma mpmc_queue_2_push_spec t ι v :
+  #[local] Lemma mpmc_queue_2_help_spec l γ backs i prev_back back move :
+    0 < length move →
+    {{{
+      meta l nroot γ ∗
+      inv' l γ ∗
+      state_lb γ backs i (Unstable back move) ∗
+      prev_back ↦ₕ Header §Back 2
+    }}}
+      mpmc_queue_2_help #l #back #⁺(S i + length move) (prefix_to_val (S i) prev_back move)
+    {{{
+      RET ();
+      True
+    }}}.
+  Proof.
+    iIntros "%Hmove %Φ (#Hmeta & #Hinv & #Hstate_lb & #Hprev_back_header) HΦ".
+
+    wp_rec. wp_pures.
+
+    wp_bind (_.{front})%E.
+    iInv "Hinv" as "(:inv_inner =1)".
+    wp_load.
+    iDestruct (state_lb_get with "Hstate_auth") as "#Hstate_lb_1".
+
+    destruct vs_front1 as [| v vs_front1'].
+
+    - rewrite right_id in Hi1. simplify.
+
+      destruct (decide (i + length move ≤ i1)) as [Hif | Hif].
+
+      + iDestruct (state_lb_stabilized with "Hstate_auth Hstate_lb") as %Hbacks1_lookup; first auto.
+
+        iSplitR "HΦ". { iFrameSteps. }
+        iModIntro. clear- Hif Hbacks1_lookup.
+
+        wp_pures.
+        rewrite bool_decide_eq_true_2; first lia.
+        wp_smart_apply (mpmc_queue_2_finish_spec with "[$] HΦ"); first done.
+
+      + iDestruct (state_lb_unstabilized with "Hstate_auth Hstate_lb") as %(-> & -> & ->); first lia.
+        iSplitR "HΦ". { iFrameSteps. }
+        iModIntro. clear- Hmove Hif.
+
+        wp_pures.
+        rewrite bool_decide_eq_false_2; first lia.
+        wp_smart_apply (mpmc_queue_2_rev_spec with "Hprev_back_header") as "_"; first lia.
+        wp_pures.
+
+        wp_bind (CAS _ _ _).
+        iInv "Hinv" as "(:inv_inner =2)".
+        wp_cas as _ | (-> & ->)%(inj2 suffix_to_val _ _ _ []).
+
+        * iSplitR "HΦ". { iFrameSteps. }
+          iSteps.
+
+        * rewrite Nat.add_0_r in Hi2. injection Hi2 as <-.
+          iDestruct (state_lb_unstabilized with "Hstate_auth Hstate_lb") as %(-> & _ & ->); first lia.
+          iDestruct "Hstatus" as "(:inv_status_unstable =2 lazy=)".
+
+          iAssert ⌜backs !! back2 = None⌝%I as %Hbacks_lookup.
+          { rewrite -eq_None_ne_Some. iIntros "%i_back %Hbacks_lookup".
+            iDestruct (big_sepM_lookup with "Hbacks") as "(:back_model_3 only_move=)"; first done.
+            iDestruct "Hback2" as "(:back_model_2 suff=)".
+            iApply (pointsto_exclusive with "Hback_move Hback_move_").
+          }
+
+          iMod (state_stabilize with "Hstate_auth") as "(Hstate_auth & #Hstatus_lb_2)"; first done.
+          iDestruct (big_sepM_insert_2 with "[Hback2] Hbacks") as "Hbacks"; first iFrameSteps.
+          iSplitR "HΦ".
+          { iFrameSteps; iPureIntro.
+            - simpl_length.
+            - rewrite lookup_insert //.
+            - rewrite right_id //.
+            - simpl_length.
+          }
+          iIntros "!> {%}".
+
+          wp_smart_apply (mpmc_queue_2_finish_spec with "[$] HΦ").
+          { rewrite lookup_insert //. }
+
+    - iAssert ⌜status1 ≠ Unstable back move⌝%I as %Hstabilized.
+      { iIntros (->).
+        iDestruct "Hstatus" as "(:inv_status_unstable =1 lazy=)". done.
+      }
+      iDestruct (state_lb_stabilized with "Hstate_auth Hstate_lb") as %Hbacks1_lookup; first auto.
+
+      iSplitR "HΦ". { iFrameSteps. }
+      iModIntro. clear- Hbacks1_lookup.
+
+      wp_smart_apply (mpmc_queue_2_finish_spec with "[$] HΦ"); first done.
+  Qed.
+
+  #[local] Lemma mpmc_queue_2_push_aux_push_spec t v ι :
+    ⊢ (
+      ∀ (i : nat) w pref,
+      <<<
+        mpmc_queue_2_inv t ι
+      | ∀∀ vs,
+        mpmc_queue_2_model t vs
+      >>>
+        mpmc_queue_2_push_aux t v #i ’Snoc( #i, w, pref ) @ ↑ι
+      <<<
+        mpmc_queue_2_model t (vs ++ [v])
+      | RET ();
+        True
+      >>>
+    ) ∧ (
+      <<<
+        mpmc_queue_2_inv t ι
+      | ∀∀ vs,
+        mpmc_queue_2_model t vs
+      >>>
+        mpmc_queue_2_push t v @ ↑ι
+      <<<
+        mpmc_queue_2_model t (vs ++ [v])
+      | RET ();
+        True
+      >>>
+    ).
+  Proof.
+  Admitted.
+  Lemma mpmc_queue_2_push_spec t v ι :
     <<<
       mpmc_queue_2_inv t ι
     | ∀∀ vs,
@@ -424,7 +956,9 @@ Section mpmc_queue_2_G.
       True
     >>>.
   Proof.
-  Admitted.
+    iDestruct mpmc_queue_2_push_aux_push_spec as "(_ & H)".
+    iApply "H".
+  Qed.
 
   Lemma mpmc_queue_2_pop_spec t ι :
     <<<
